theories/region_invariants.v
@@ -41,7 +41,7 @@ Class heapGpreS Σ {Cname : CmptNameG} := HeapGpreS {
   heapPreG_invPreG : invGpreS Σ;
   heapPreG_saved_pred ::
     savedPredG Σ (
-      (gmap CmptName ((STS_std_states Addr region_type) * (STS_states * STS_rels))) *
+      ((STS_std_states Addr region_type) * (STS_states * STS_rels)) *
         CmptName *
         Word);
   heapPreG_rel :: inG Σ (authR relUR);
@@ -50,7 +50,7 @@ Class heapGpreS Σ {Cname : CmptNameG} := HeapGpreS {
 Class heapGS Σ {Cname : CmptNameG} := HeapGS {
   heapG_saved_pred ::
     savedPredG Σ (
-      (gmap CmptName ((STS_std_states Addr region_type) * (STS_states * STS_rels))) *
+      ((STS_std_states Addr region_type) * (STS_states * STS_rels)) *
         CmptName *
         Word);
   heapG_rel :: inG Σ (authR relUR);
@@ -64,7 +64,7 @@ Instance subG_heapPreΣ {Σ} {Cname : CmptNameG}:
   subG heapPreΣ Σ →
   invGpreS Σ →
   subG (savedPredΣ
-          ((gmap CmptName ((STS_std_states Addr region_type) * (STS_states * STS_rels))) *
+          ((((STS_std_states Addr region_type) * (STS_states * STS_rels))) *
         CmptName *
         Word)) Σ →
   heapGpreS Σ.
@@ -86,7 +86,7 @@ Section REL_defs.
   Definition RELS_eq : @RELS = @RELS_def := proj2_sig RELS_aux.
 
   Definition rel_def (C : CmptName) (a : Addr) (p : Perm)
-    (φ : ((gmap CmptName ((STS_std_states Addr region_type) * (STS_states * STS_rels))) *
+    (φ : (((STS_std_states Addr region_type) * (STS_states * STS_rels)) *
         CmptName *
         Word) -> iProp Σ)
     : iProp Σ :=
@@ -143,9 +143,7 @@ Section heap.
     `{MP: MachineParameters}.
   Notation STS := (leibnizO (STS_states * STS_rels)).
   Notation STS_STD := (leibnizO (STS_std_states Addr region_type)).
-  Notation CVIEW := (prodO STS_STD STS).
-  Notation WORLD := (gmapO CmptName CVIEW).
-  Implicit Types WC : CVIEW.
+  Notation WORLD := (prodO STS_STD STS).
   Implicit Types W : WORLD.
 
   Global Instance region_type_EqDecision : EqDecision region_type :=
@@ -194,12 +192,12 @@ Section heap.
 
   Definition future_pub_mono (C : CmptName) (φ : (WORLD * CmptName * Word) -> iProp Σ) (v  : Word) : iProp Σ :=
     (□ ∀ (W W' : WORLD),
-        ⌜ related_sts_pub_world W W' C ⌝
+        ⌜ related_sts_pub_world W W'⌝
         → φ (W,C,v) -∗ φ (W',C,v))%I.
 
   Definition future_priv_mono (C : CmptName) (φ : (WORLD * CmptName * Word) -> iProp Σ) (v  : Word) : iProp Σ :=
     (□ ∀ (W W' : WORLD),
-        ⌜ related_sts_priv_world W W' C⌝
+        ⌜ related_sts_priv_world W W'⌝
         → φ (W,C,v) -∗ φ (W',C,v))%I.
 
   Lemma future_priv_mono_is_future_pub_mono (C : CmptName) (φ: (WORLD * CmptName * Word) → iProp Σ) v :
@@ -274,46 +272,25 @@ Section heap.
 
   (* Asserting that a location is in a specific state in a given World *)
 
-  Definition permanent_cview (WC : CVIEW) (a : Addr) :=
-    match (std_cview WC) !! a with
+  Definition permanent (W : WORLD) (a : Addr) :=
+    match (std W) !! a with
     | Some ρ => ρ = Permanent
     | _ => False
     end.
-  Definition revoked_cview (WC : CVIEW) (a : Addr) :=
-    match (std_cview WC) !! a with
+  Definition revoked (W : WORLD) (a : Addr) :=
+    match (std W) !! a with
     | Some ρ => ρ = Revoked
     | _ => False
     end.
-  Definition frozen_cview (WC : CVIEW) (m: gmap Addr Word) (a : Addr) :=
-    match (std_cview WC) !! a with
+  Definition frozen (W : WORLD) (m: gmap Addr Word) (a : Addr) :=
+    match (std W) !! a with
     | Some ρ => ρ = (Frozen m)
     | _ => False
     end.
-  Definition temporary_cview (WC : CVIEW) (a : Addr) :=
-    match (std_cview WC) !! a with
+  Definition temporary (W : WORLD) (a : Addr) :=
+    match (std W) !! a with
     | Some ρ => ρ = Temporary
     | _ => False
-    end.
-
-  Definition permanent (W : WORLD) (C : CmptName) (a : Addr) :=
-    match W !! C with
-    | Some WC => permanent_cview WC a
-    | None => False
-    end.
-  Definition revoked (W : WORLD) (C : CmptName) (a : Addr) :=
-    match W !! C with
-    | Some WC => revoked_cview WC a
-    | None => False
-    end.
-  Definition frozen (W : WORLD) (C : CmptName) (m: gmap Addr Word) (a : Addr) :=
-    match W !! C with
-    | Some WC => frozen_cview WC m a
-    | None => False
-    end.
-  Definition temporary (W : WORLD) (C : CmptName) (a : Addr) :=
-    match W !! C with
-    | Some WC => temporary_cview WC a
-    | None => False
     end.
 
   (* ----------------------------------------------------------------------------------------------- *)
@@ -355,7 +332,7 @@ Section heap.
   Definition region_def (W : WORLD) (C : CmptName) : iProp Σ :=
     (∃ (M : relT) (Mρ: gmap Addr region_type),
         RELS C M
-        ∗ ⌜dom (std W C) = dom M⌝
+        ∗ ⌜dom (std W) = dom M⌝
         ∗ ⌜dom Mρ = dom M⌝
         ∗ region_map_def W C M Mρ)%I.
   Definition region_aux : { x | x = @region_def }. by eexists. Qed.
@@ -409,7 +386,7 @@ Section heap.
   Qed.
 
   Lemma region_rel_get (W : WORLD) (C : CmptName) (a : Addr) :
-    (std W C) !! a = Some Temporary ->
+    (std W) !! a = Some Temporary ->
     region W C ∗ sts_full_world W C
     ==∗
     region W C ∗ sts_full_world W C ∗ ∃ p φ, ⌜forall WCv, Persistent (φ WCv)⌝ ∗ rel C a p φ.
@@ -424,8 +401,7 @@ Section heap.
     iMod (reg_get with "[$HM]") as "[HM Hrel]";[eauto|].
     iDestruct (big_sepM_delete _ _ a with "Hr") as "[Hstate Hr]";[eauto|].
     iDestruct "Hstate" as (ρ Ha) "[Hρ Hstate]".
-    iDestruct (sts_full_state_std with "Hsts Hρ") as %(WC & HWC & Hx''); simplify_eq.
-    all: rewrite /std HWC in Hlookup .
+    iDestruct (sts_full_state_std with "Hsts Hρ") as %Hx''; simplify_eq.
     all: rewrite Hlookup in Hx'';inversion Hx'';subst.
     all: iDestruct "Hstate" as (γpred p' φ Heq Hpers) "(#Hsaved & Ha)".
     all: iDestruct "Ha" as (v Hne) "(Ha & #HmonoV & #Hφ)".
@@ -560,7 +536,7 @@ Section heap.
   (* region_map is monotone with regards to public future world relation *)
 
   Lemma region_map_monotone (C : CmptName) (W W' : WORLD) M Mρ :
-    related_sts_pub_world W W' C
+    related_sts_pub_world W W'
     → region_map_def W C M Mρ
     -∗ region_map_def W' C M Mρ.
   Proof.
@@ -587,13 +563,12 @@ Section heap.
   Qed.
 
   Lemma region_monotone C W W':
-    dom W = dom W'
-    -> dom (std W C)= dom (std W' C)
-    -> related_sts_pub_world W W' C
+    dom (std W) = dom (std W')
+    -> related_sts_pub_world W W'
     → region W C
     -∗ region W' C.
   Proof.
-    iIntros (HdomW Hdomeq Hrelated) "HW". rewrite region_eq.
+    iIntros (Hdomeq Hrelated) "HW". rewrite region_eq.
     iDestruct "HW" as (M Mρ) "(HM & % & % & Hmap)"; simplify_map_eq.
     iExists M, Mρ. iFrame.
     repeat(iSplitR; auto).
@@ -601,9 +576,9 @@ Section heap.
     - iApply region_map_monotone; last eauto;eauto.
   Qed.
 
-  Lemma uninitialized_mono_related_sts_pub_cview WC a w :
-    (std_cview WC) !! a = Some (Frozen {[a:=w]}) ->
-    related_sts_pub_cview WC (<s[ a := Temporary ]s> WC).
+  Lemma uninitialized_mono_related_sts_pub_world W a w :
+    (std W) !! a = Some (Frozen {[a:=w]}) ->
+    related_sts_pub_world W (<s[ a := Temporary ]s> W).
   Proof.
     intros.
     split;[|apply related_sts_pub_refl].
@@ -611,26 +586,13 @@ Section heap.
     - rewrite dom_insert_L. set_solver.
     - intros i x y Hx Hy.
       destruct (decide (i = a)).
-      + subst. rewrite /std_cview in H.
+      + subst. rewrite /std in H.
         simplify_map_eq. rewrite H in Hx.
         inv Hx.
         right with Temporary;constructor.
       + simplify_map_eq; auto.
         rewrite Hx in Hy.
         simplify_eq. left.
-  Qed.
-
-  Lemma uninitialized_mono_related_sts_pub_world W C a w :
-    (std W C) !! a = Some (Frozen {[a:=w]}) ->
-    related_sts_pub_world W (<s[ (C,a) := Temporary ]s> W) C.
-  Proof.
-    rewrite /std /related_sts_pub_world.
-    intros.
-    destruct (W !! C) as [WC|] eqn:HWC ; last by simplify_map_eq.
-    rewrite !/std_update HWC dom_insert_L lookup_insert.
-    split; first set_solver.
-    intros WC0 WC' ? HWC'; simplify_eq.
-    eapply uninitialized_mono_related_sts_pub_cview; eauto.
   Qed.
 
   (* Lemma uninitialized_w_mono_related_sts_pub_world l W w : *)
@@ -656,7 +618,7 @@ Section heap.
   Definition open_region_def (W : WORLD) (C : CmptName) (a : Addr) : iProp Σ :=
     (∃ (M : relT) (Mρ: gmap Addr region_type),
         RELS C M
-        ∗ ⌜dom (std W C) = dom M⌝
+        ∗ ⌜dom (std W) = dom M⌝
         ∗ ⌜dom Mρ = dom M⌝
         ∗ region_map_def W C (delete a M) (delete a Mρ))%I.
   Definition open_region_aux : { x | x = @open_region_def }. by eexists. Qed.
@@ -665,13 +627,12 @@ Section heap.
 
   (* open_region is monotone wrt public future worlds *)
   Lemma open_region_monotone C W W' a :
-    dom W = dom W'
-    -> dom (std W C) = dom (std W' C)
-    -> related_sts_pub_world W W' C
+    dom (std W)  = dom (std W')
+    -> related_sts_pub_world W W'
     → open_region W C a
     -∗ open_region W' C a.
   Proof.
-    iIntros (HdomW Hdomeq Hrelated) "HW". rewrite open_region_eq /open_region_def.
+    iIntros (Hdomeq Hrelated) "HW". rewrite open_region_eq /open_region_def.
     iDestruct "HW" as (M Mρ) "(HM & % & % & Hmap)"; simplify_map_eq.
     iExists M, Mρ. iFrame.
     repeat(iSplitR; auto).
@@ -728,7 +689,7 @@ Section heap.
   Qed.
 
   Lemma region_open_temp_pwl W C l p φ :
-    (std W C) !! l = Some Temporary →
+    (std W) !! l = Some Temporary →
     isWL p = true →
     rel C l p φ ∗ region W C ∗ sts_full_world W C -∗
     ∃ v, open_region W C l
@@ -748,8 +709,7 @@ Section heap.
     rewrite HMeq big_sepM_insert; [|by rewrite lookup_delete].
     iDestruct "Hpreds" as "[Hl Hpreds]".
     iDestruct "Hl" as (ρ Hρ) "[Hstate Hl]".
-    iDestruct (sts_full_state_std with "Hfull Hstate") as %(WC & HWC & Hst).
-    rewrite /std HWC in Htemp.
+    iDestruct (sts_full_state_std with "Hfull Hstate") as %Hst.
     rewrite Htemp in Hst. (destruct ρ; try by simplify_eq); [].
     iDestruct "Hl" as (γpred' p' φ' HH1 Hpers) "(#Hφ' & Hl)".
     iDestruct "Hl" as (v Hne) "(Hl & #HmonoV & Hφv)".
@@ -770,7 +730,7 @@ Section heap.
 
 
   Lemma region_open_temp_nwl W C l p φ :
-    (std W C) !! l = Some Temporary →
+    (std W) !! l = Some Temporary →
     isWL p = false →
     rel C l p φ ∗ region W C ∗ sts_full_world W C -∗
         ∃ v, open_region W C l
@@ -790,8 +750,7 @@ Section heap.
     rewrite HMeq big_sepM_insert; [|by rewrite lookup_delete].
     iDestruct "Hpreds" as "[Hl Hpreds]".
     iDestruct "Hl" as (ρ Hρ) "[Hstate Hl]".
-    iDestruct (sts_full_state_std with "Hfull Hstate") as %(WC & HWC & Hst).
-    rewrite /std HWC in Htemp.
+    iDestruct (sts_full_state_std with "Hfull Hstate") as %Hst.
     rewrite Htemp in Hst. (destruct ρ; try by simplify_eq); [].
     iDestruct "Hl" as (γpred' p' φ' HH Hpers) "(#Hφ' & Hl)".
     iDestruct "Hl" as (v Hne) "(Hl & #HmonoV & Hφv)".
@@ -855,7 +814,7 @@ Section heap.
   (* Qed. *)
 
     Lemma region_open_perm W C l p φ :
-    (std W C) !! l = Some Permanent →
+    (std W) !! l = Some Permanent →
     rel C l p φ ∗ region W C ∗ sts_full_world W C -∗
         ∃ v, open_region W C l
            ∗ sts_full_world W C
@@ -874,8 +833,7 @@ Section heap.
     rewrite HMeq big_sepM_insert; [|by rewrite lookup_delete].
     iDestruct "Hpreds" as "[Hl Hpreds]".
     iDestruct "Hl" as (ρ Hρ) "[Hstate Hl]".
-    iDestruct (sts_full_state_std with "Hfull Hstate") as %(WC & HWC & Hst).
-    rewrite /std HWC in Htemp.
+    iDestruct (sts_full_state_std with "Hfull Hstate") as %Hst.
     rewrite Htemp in Hst. (destruct ρ; try by simplify_eq); [].
     iDestruct "Hl" as (γpred' p' φ' HH Hpers) "(#Hφ' & Hl)".
     iDestruct "Hl" as (v Hne) "(Hl & #HmonoV & Hφv)".
@@ -924,7 +882,7 @@ Section heap.
 
   Lemma region_open W C a p φ (ρ : region_type) :
     ρ = Temporary ∨ ρ = Permanent →
-    (std W C) !! a = Some ρ →
+    (std W) !! a = Some ρ →
     rel C a p φ ∗ region W C ∗ sts_full_world W C -∗
     ∃ v, open_region W C a
          ∗ sts_full_world W C
@@ -1019,41 +977,39 @@ Section heap.
 
   Lemma full_sts_Mρ_agree W C M Mρ (ρ: region_type) :
     (* NB: only the forward direction of dom_equal (std_sta W) M is actually needed *)
-    dom (std W C) = dom M →
+    dom (std W) = dom M →
     (* NB: only one direction of this assumption is needed, and only for the reverse *)
   (*      direction of the lemma *)
     dom Mρ = dom M →
     sts_full_world W C -∗
     region_map_def W C M Mρ -∗
-    ⌜∀ a:Addr, (std W C) !! a = Some ρ ↔ Mρ !! a = Some ρ⌝.
+    ⌜∀ a:Addr, (std W) !! a = Some ρ ↔ Mρ !! a = Some ρ⌝.
   Proof.
     iIntros (HWM HMMρ) "Hfull Hr".
-    iAssert (∀ a:Addr, ⌜ (std W C) !! a = Some ρ ⌝ → ⌜ Mρ !! a = Some ρ ⌝)%I as %?.
+    iAssert (∀ a:Addr, ⌜ (std W) !! a = Some ρ ⌝ → ⌜ Mρ !! a = Some ρ ⌝)%I as %?.
     { iIntros (a Haρ).
       assert (is_Some (M !! a)) as [γp Hγp].
       { apply elem_of_dom.
-        rewrite -HWM. apply (elem_of_dom (std W C)) . eauto. }
+        rewrite -HWM. apply (elem_of_dom (std W)) . eauto. }
       iDestruct (big_sepM_lookup with "Hr") as (ρ' Hρ') "(Hst & _)"; eauto; [].
-      iDestruct (sts_full_state_std with "Hfull Hst") as %(WC & HWC & Haρ').
-      rewrite /std HWC in Haρ.
+      iDestruct (sts_full_state_std with "Hfull Hst") as %Haρ'.
       enough (ρ = ρ') by (subst; eauto). apply encode_inj.
       rewrite Haρ in Haρ'. congruence. }
-    iAssert (∀ a:Addr, ⌜ Mρ !! a = Some ρ ⌝ → ⌜ (std W C) !! a = Some ρ ⌝)%I as %?.
+    iAssert (∀ a:Addr, ⌜ Mρ !! a = Some ρ ⌝ → ⌜ (std W) !! a = Some ρ ⌝)%I as %?.
     { iIntros (a HMρa).
       assert (is_Some (M !! a)) as [γp Hγp].
       { rewrite -elem_of_dom -HMMρ elem_of_dom; eauto. }
       iDestruct (big_sepM_lookup with "Hr") as (ρ' Hρ') "(Hst & _)"; eauto; [].
-      iDestruct (sts_full_state_std with "Hfull Hst") as %(WC & HWC & Haρ').
-      rewrite /std HWC.
+      iDestruct (sts_full_state_std with "Hfull Hst") as %Haρ'.
       enough (ρ = ρ') by (subst; eauto). rewrite HMρa in Hρ'. congruence. }
     iPureIntro. intros. split; eauto.
   Qed.
 
   Lemma full_sts_frozen_all W C m (a : Addr) :
-    (std W C) !! a = Some (Frozen m) →
+    (std W) !! a = Some (Frozen m) →
     sts_full_world W C -∗
     region W C -∗
-    ⌜forall a', a' ∈ dom m -> frozen W C m a'⌝.
+    ⌜forall a', a' ∈ dom m -> frozen W m a'⌝.
   Proof.
     iIntros (Hfrozen) "Hsts Hr".
     rewrite region_eq /region_def.
@@ -1077,12 +1033,10 @@ Section heap.
     iPureIntro.
     rewrite /std in Hfrozen.
     rewrite /frozen.
-    destruct (W !!C) as [WC|] eqn:HWC; last done.
     destruct (Hag' a') as [_ Hag2].
     pose proof (Hall _ Hdom) as Ha.
     pose proof (Hag2 Ha) as Hf.
-    rewrite /std HWC in Hf.
-    by rewrite /frozen_cview Hf.
+    by rewrite Hf.
   Qed.
 
    (* Closing the region without updating the sts collection *)
@@ -1255,7 +1209,7 @@ Section heap.
   Definition open_region_many_def  (W : WORLD) (C : CmptName) (l : list Addr) : iProp Σ :=
     (∃ (M : relT) (Mρ: gmap Addr region_type),
         RELS C M
-        ∗ ⌜dom (std W C) = dom M⌝
+        ∗ ⌜dom (std W) = dom M⌝
         ∗ ⌜dom Mρ = dom M⌝
         ∗ region_map_def W C (delete_list l M) (delete_list l Mρ))%I.
   Definition open_region_many_aux : { x | x = @open_region_many_def }. by eexists. Qed.
@@ -1263,12 +1217,11 @@ Section heap.
   Definition open_region_many_eq : @open_region_many = @open_region_many_def := proj2_sig open_region_many_aux.
 
   Lemma open_region_many_monotone (C : CmptName) (W W' : WORLD) l:
-    dom W = dom W'
-    -> dom (std W C) = dom (std W' C)
-    -> related_sts_pub_world W W' C
+    dom (std W) = dom (std W')
+    -> related_sts_pub_world W W'
     -> open_region_many W C l -∗ open_region_many W' C l.
   Proof.
-    iIntros (HdomW Hdomeq Hrelated) "HW".
+    iIntros (Hdomeq Hrelated) "HW".
     rewrite open_region_many_eq /open_region_many_def.
     iDestruct "HW" as (M Mρ) "(Hm & % & % & Hmap)" ; simplify_eq.
     iExists M, Mρ. iFrame.
@@ -1304,7 +1257,7 @@ Section heap.
 
   Lemma region_open_next_temp_pwl W C φ als a p :
     a ∉ als →
-    (std W C) !! a = Some Temporary ->
+    (std W) !! a = Some Temporary ->
     isWL p = true →
     open_region_many W C als ∗ rel C a p φ ∗ sts_full_world W C -∗
     ∃ v, open_region_many W C (a :: als)
@@ -1327,8 +1280,7 @@ Section heap.
     rewrite HMeq big_sepM_insert; [|by rewrite lookup_delete].
     iDestruct "Hpreds" as "[Hl Hpreds]".
     iDestruct "Hl" as (ρ Hρ) "[Hstate Hl]".
-    iDestruct (sts_full_state_std with "Hfull Hstate") as %(WC & HWC & Hst).
-    rewrite /std HWC in Htemp.
+    iDestruct (sts_full_state_std with "Hfull Hstate") as %Hst.
     rewrite Htemp in Hst. (destruct ρ; try by simplify_eq); [].
     iDestruct "Hl" as (γpred' p' φ' HH Hpers) "(#Hφ' & Hl)".
     iDestruct "Hl" as (v Hne) "(Hl & #HmonoV & Hφv)".
@@ -1347,7 +1299,7 @@ Section heap.
 
   Lemma region_open_next_temp_nwl W C φ als a p :
     a ∉ als →
-    (std W C) !! a = Some Temporary ->
+    (std W) !! a = Some Temporary ->
     isWL p = false →
     open_region_many W C als ∗ rel C a p φ ∗ sts_full_world W C -∗
     ∃ v, open_region_many W C (a :: als)
@@ -1370,8 +1322,7 @@ Section heap.
     rewrite HMeq big_sepM_insert; [|by rewrite lookup_delete].
     iDestruct "Hpreds" as "[Hl Hpreds]".
     iDestruct "Hl" as (ρ Hρ) "[Hstate Hl]".
-    iDestruct (sts_full_state_std with "Hfull Hstate") as %(WC & HWC & Hst).
-    rewrite /std HWC in Htemp.
+    iDestruct (sts_full_state_std with "Hfull Hstate") as %Hst.
     rewrite Htemp in Hst. (destruct ρ; try by simplify_eq); [].
     iDestruct "Hl" as (γpred' p' φ' HH Hpers) "(#Hφ' & Hl)".
     iDestruct "Hl" as (v Hne) "(Hl & #HmonoV & Hφv)".
@@ -1389,7 +1340,7 @@ Section heap.
   Qed.
 
   Lemma region_open_next_perm W C φ als a p :
-    a ∉ als → (std W C) !! a = Some Permanent ->
+    a ∉ als → (std W) !! a = Some Permanent ->
     open_region_many W C als
     ∗ rel C a p φ
     ∗ sts_full_world W C
@@ -1414,8 +1365,7 @@ Section heap.
     rewrite HMeq big_sepM_insert; [|by rewrite lookup_delete].
     iDestruct "Hpreds" as "[Hl Hpreds]".
     iDestruct "Hl" as (ρ Hρ) "[Hstate Hl]".
-    iDestruct (sts_full_state_std with "Hfull Hstate") as %(WC & HWC & Hst).
-    rewrite /std HWC in Htemp.
+    iDestruct (sts_full_state_std with "Hfull Hstate") as %Hst.
     rewrite Htemp in Hst. (destruct ρ; try by simplify_eq); [].
     iDestruct "Hl" as (γpred' p' φ' HH Hpers) "(#Hφ' & Hl)".
     iDestruct "Hl" as (v Hne) "(Hl & #HmonoV & Hφv)".
@@ -1435,7 +1385,7 @@ Section heap.
 
   Lemma region_open_next_uninit W C w als a:
     a ∉ als →
-    (std W C) !! a = Some (Frozen {[a:=w]}) →
+    (std W) !! a = Some (Frozen {[a:=w]}) →
     open_region_many W C als ∗ sts_full_world W C -∗
         ∃ p, open_region_many W C (a :: als)
            ∗ sts_full_world W C
@@ -1452,8 +1402,7 @@ Section heap.
     { rewrite lookup_delete_list_notin; eauto. }
     iDestruct "Hl" as (ρ) "[% [Hstate Hl] ]". destruct ρ.
     1,2,3,4:
-      iDestruct (sts_full_state_std with "Hfull Hstate") as %(WC & HWC & Hcontr)
-          ; rewrite /std HWC in Htemp.
+      iDestruct (sts_full_state_std with "Hfull Hstate") as %Hcontr.
     1,2,3: rewrite Htemp in Hcontr; by inversion Hcontr.
     iDestruct "Hl" as (γpred p φ Heq Hpers) "[#Hsaved Hl]".
     iDestruct "Hl" as (v Hne Hlookup) "[Hl _]".
@@ -1693,7 +1642,7 @@ Section heap.
     (Hρnotrevoked : ρ <> Revoked)
     (Hρnotfrozen : ¬ exists g, ρ = Frozen g):
     a ∉ als →
-    std W C !! a = Some ρ →
+    std W !! a = Some ρ →
     ⊢ open_region_many W C als
     ∗ rel C a p φ
     ∗ sts_full_world W C
@@ -1746,8 +1695,8 @@ Section heap.
   Qed.
 
   Lemma frozen_extend_preserve W (C : CmptName) (M : gmap Addr (gname*Perm)) (Mρ : gmap Addr region_type) (a : Addr) g ρ :
-    a ∉ dom (std W C) ->
-    dom (std W C) = dom M ->
+    a ∉ dom (std W) ->
+    dom (std W) = dom M ->
     dom Mρ = dom M ->
     (∀ a' : Addr, a' ∈ dom g → Mρ !! a' = Some (Frozen g)) ->
     ∀ a' : Addr, a' ∈ dom g → <[a:=ρ]> Mρ !! a' = Some (Frozen g).
@@ -1756,15 +1705,15 @@ Section heap.
     intros a' Hin. pose proof (Hall _ Hin) as Hcontr.
     assert (a' ∈ dom Mρ) as Hincontr;[apply elem_of_dom;eauto|].
     rewrite Hdom2 in Hincontr. apply elem_of_dom in Hincontr. clear Hcontr.
-    assert (is_Some (std W C !! a')) as Hcontr.
+    assert (is_Some (std W !! a')) as Hcontr.
     { rewrite -elem_of_dom. rewrite Hdom1. rewrite elem_of_dom. eauto. }
     rewrite -elem_of_dom in Hcontr.
     assert (a' ≠ a) as Hne';[intros Heq;subst;contradiction|].
     rewrite lookup_insert_ne;auto.
   Qed.
 
-  Lemma related_sts_priv_world_fresh_Permanent W C a :
-    related_sts_priv_world W (<s[(C,a):=Permanent]s> W) C.
+  Lemma related_sts_priv_world_fresh_Permanent W a :
+    related_sts_priv_world W (<s[a:=Permanent]s> W).
   Proof.
     apply related_sts_priv_world_fresh.
     intros ρ'; destruct ρ'.
