theories/ftlr/JmpCap.v
@@ -17,9 +17,7 @@ Section fundamental.
 
   Notation STS := (leibnizO (STS_states * STS_rels)).
   Notation STS_STD := (leibnizO (STS_std_states Addr region_type)).
-  Notation CVIEW := (prodO STS_STD STS).
-  Notation WORLD := (gmapO CmptName CVIEW).
-  Implicit Types WC : CVIEW.
+  Notation WORLD := (prodO STS_STD STS).
   Implicit Types W : WORLD.
   Implicit Types C : CmptName.
 
@@ -81,7 +79,7 @@ Section fundamental.
           iEval (rewrite fixpoint_interp1_eq) in "Hwsrc".
           simpl; rewrite /enter_cond.
           iDestruct "Hwsrc" as "#H".
-          iAssert (future_world g0 W W C) as "Hfuture".
+          iAssert (future_world g0 W W) as "Hfuture".
           { iApply futureworld_refl. }
           iSpecialize ("H" with "Hfuture").
           iDestruct "H" as "[H _]".
